vale/code/arch/x64/Vale.X64.QuickCodes.fsti
@@ -63,6 +63,8 @@ noeq type quickCodes (a:Type0) : codes -> Type =
     (unit -> Lemma (requires pre) (ensures post ())) -> quickCodes a cs -> quickCodes a cs
 | QGhost: #cs:codes -> b:Type -> r:range -> msg:string -> pre:Type0 -> post:(b -> Type0) ->
     (unit -> Ghost b (requires pre) (ensures post)) -> (b -> GTot (quickCodes a cs)) -> quickCodes a ((Block [])::cs)
+| QAssertBy: #cs:codes -> r:range -> msg:string -> p:Type0 ->
+    quickCodes unit [] -> quickCodes a cs -> quickCodes a cs
 
 [@va_qattr]
 let qPURE
@@ -88,9 +90,13 @@ let wp_proc (#a:Type0) (c:code) (qc:quickCode a c) (s0:vale_state) (k:vale_state
 
 let wp_Seq_t (a:Type0) = vale_state -> a -> Type0
 let wp_Bind_t (a:Type0) = vale_state -> a -> Type0
+let k_AssertBy (p:Type0) (_:vale_state) () = p
 
 [@va_qattr]
 let range1 = mk_range "" 0 0 0 0
+
+val empty_list_is_small (#a:Type) (x:list a) : Lemma
+  ([] #a == x \/ [] #a << x)
 
 [@va_qattr]
 let rec wp (#a:Type0) (cs:codes) (qcs:quickCodes a cs) (mods:mods_t) (k:vale_state -> a -> Type0) (s0:vale_state) :
@@ -129,6 +135,9 @@ let rec wp (#a:Type0) (cs:codes) (qcs:quickCodes a cs) (mods:mods_t) (k:vale_sta
   | QGhost b r msg pre post l qcs ->
       let c::cs = cs in
       label r msg pre /\ (forall (g:b). post g ==> wp cs (qcs g) mods k s0)
+  | QAssertBy r msg p qcsBy qcs ->
+      empty_list_is_small cs;
+      wp [] qcsBy mods (k_AssertBy p) s0 /\ (p ==> wp cs qcs mods k s0)
 // Hoist lambdas out of main definition to avoid issues with function equality
 and wp_Seq (#a:Type0) (#b:Type0) (cs:codes) (qcs:quickCodes b cs) (mods:mods_t) (k:vale_state -> b -> Type0) :
   Tot (wp_Seq_t a) (decreases %[cs; 1; qcs])
@@ -141,9 +150,9 @@ and wp_Bind (#a:Type0) (#b:Type0) (cs:codes) (qcs:vale_state -> a -> GTot (quick
 
 val wp_sound (#a:Type0) (cs:codes) (qcs:quickCodes a cs) (mods:mods_t) (k:vale_state -> a -> Type0) (s0:vale_state)
   : Ghost (vale_state & va_fuel & a)
-  (requires wp cs qcs mods k s0)
+  (requires t_require s0 /\ wp cs qcs mods k s0)
   (ensures fun (sN, fN, gN) ->
-    eval (Block cs) s0 fN sN /\ update_state_mods mods sN s0 == sN /\ k sN gN
+    eval (Block cs) s0 fN sN /\ update_state_mods mods sN s0 == sN /\ state_inv sN /\ k sN gN
   )
 
 ///// Block
@@ -156,9 +165,9 @@ let wp_block (#a:Type) (#cs:codes) (qcs:vale_state -> GTot (quickCodes a cs)) (m
 
 val qblock_proof (#a:Type) (#cs:codes) (qcs:vale_state -> GTot (quickCodes a cs)) (mods:mods_t) (s0:vale_state) (k:vale_state -> a -> Type0)
   : Ghost (vale_state & va_fuel & a)
-  (requires wp_block qcs mods s0 k)
+  (requires t_require s0 /\ wp_block qcs mods s0 k)
   (ensures fun (sM, f0, g) ->
-    eval_code (block cs) s0 f0 sM /\ update_state_mods mods sM s0 == sM /\ k sM g
+    eval_code (block cs) s0 f0 sM /\ update_state_mods mods sM s0 == sM /\ state_inv sM /\ k sM g
   )
 
 [@"opaque_to_smt" va_qattr]
@@ -175,9 +184,9 @@ let wp_InlineIf (#a:Type) (#c1:code) (#c2:code) (b:bool) (qc1:quickCode a c1) (q
 
 val qInlineIf_proof (#a:Type) (#c1:code) (#c2:code) (b:bool) (qc1:quickCode a c1) (qc2:quickCode a c2) (mods:mods_t) (s0:vale_state) (k:vale_state -> a -> Type0)
   : Ghost (vale_state & va_fuel & a)
-  (requires wp_InlineIf b qc1 qc2 mods s0 k)
+  (requires t_require s0 /\ wp_InlineIf b qc1 qc2 mods s0 k)
   (ensures fun (sM, f0, g) ->
-    eval_code (if_code b c1 c2) s0 f0 sM /\ update_state_mods mods sM s0 == sM /\ k sM g
+    eval_code (if_code b c1 c2) s0 f0 sM /\ update_state_mods mods sM s0 == sM /\ state_inv sM /\ k sM g
   )
 
 [@"opaque_to_smt" va_qattr]
@@ -231,9 +240,9 @@ let wp_If (#a:Type) (#c1:code) (#c2:code) (b:cmp) (qc1:quickCode a c1) (qc2:quic
 
 val qIf_proof (#a:Type) (#c1:code) (#c2:code) (b:cmp) (qc1:quickCode a c1) (qc2:quickCode a c2) (mods:mods_t) (s0:vale_state) (k:vale_state -> a -> Type0)
   : Ghost (vale_state & va_fuel & a)
-  (requires wp_If b qc1 qc2 mods s0 k)
+  (requires t_require s0 /\ wp_If b qc1 qc2 mods s0 k)
   (ensures fun (sM, f0, g) ->
-    eval_code (IfElse (cmp_to_ocmp b) c1 c2) s0 f0 sM /\ update_state_mods mods sM s0 == sM /\ k sM g
+    eval_code (IfElse (cmp_to_ocmp b) c1 c2) s0 f0 sM /\ update_state_mods mods sM s0 == sM /\ state_inv sM /\ k sM g
   )
 
 [@"opaque_to_smt" va_qattr]
@@ -271,9 +280,9 @@ val qWhile_proof
     (#a #d:Type) (#c:code) (b:cmp) (qc:a -> quickCode a c) (mods:mods_t) (inv:vale_state -> a -> Type0)
     (dec:vale_state -> a -> d) (g0:a) (s0:vale_state) (k:vale_state -> a -> Type0)
   : Ghost (vale_state & va_fuel & a)
-  (requires wp_While b qc mods inv dec g0 s0 k)
+  (requires t_require s0 /\ wp_While b qc mods inv dec g0 s0 k)
   (ensures fun (sM, f0, g) ->
-    eval_code (While (cmp_to_ocmp b) c) s0 f0 sM /\ update_state_mods mods sM s0 == sM /\ k sM g
+    eval_code (While (cmp_to_ocmp b) c) s0 f0 sM /\ update_state_mods mods sM s0 == sM /\ state_inv sM /\ k sM g
   )
 
 [@"opaque_to_smt" va_qattr]
@@ -309,20 +318,24 @@ let qAssertSquash
   : quickCodes a ((Block [])::cs) =
   QGhost (squash e) r msg e (fun () -> e) (qAssertSquashLemma e) qcs
 
-let tAssertByLemma (#a:Type) (p:Type0) (qcs:quickCodes a []) (mods:mods_t) (s0:vale_state) =
-  unit -> Lemma (requires wp [] qcs mods (fun _ _ -> p) s0) (ensures p)
-val qAssertByLemma (#a:Type) (p:Type0) (qcs:quickCodes a []) (mods:mods_t) (s0:vale_state) : tAssertByLemma p qcs mods s0
+//let tAssertByLemma (#a:Type) (p:Type0) (qcs:quickCodes a []) (mods:mods_t) (s0:state) =
+//  unit -> Lemma (requires t_require s0 /\ wp [] qcs mods (fun _ _ -> p) s0) (ensures p)
+//val qAssertByLemma (#a:Type) (p:Type0) (qcs:quickCodes a []) (mods:mods_t) (s0:state) : tAssertByLemma p qcs mods s0
+//
+//[@va_qattr]
+//let qAssertBy (#a:Type) (#cs:codes) (mods:mods_t) (r:range) (msg:string) (p:Type0) (qcsBy:quickCodes unit []) (s0:state) (qcsTail:quickCodes a cs) : quickCodes a cs =
+//  QLemma r msg (t_require s0 /\ wp [] qcsBy mods (fun _ _ -> p) s0) (fun () -> p) (qAssertByLemma p qcsBy mods s0) qcsTail
 
 [@va_qattr]
-let qAssertBy (#a:Type) (#cs:codes) (mods:mods_t) (r:range) (msg:string) (p:Type0) (qcsBy:quickCodes unit []) (s0:vale_state) (qcsTail:quickCodes a cs) : quickCodes a cs =
-  QLemma r msg (wp [] qcsBy mods (fun _ _ -> p) s0) (fun () -> p) (qAssertByLemma p qcsBy mods s0) qcsTail
+let qAssertBy (#a:Type) (#cs:codes) (r:range) (msg:string) (p:Type0) (qcsBy:quickCodes unit []) (qcsTail:quickCodes a cs) : quickCodes a cs =
+  QAssertBy r msg p qcsBy qcsTail
 
 ///// Code
 
 val wp_sound_code (#a:Type0) (c:code) (qc:quickCode a c) (k:vale_state -> a -> Type0) (s0:vale_state) :
   Ghost (vale_state & fuel & a)
-  (requires QProc?.wp qc s0 k)
-  (ensures fun (sN, fN, gN) -> eval_code c s0 fN sN /\ update_state_mods qc.mods sN s0 == sN /\ k sN gN)
+  (requires t_require s0 /\ QProc?.wp qc s0 k)
+  (ensures fun (sN, fN, gN) -> eval_code c s0 fN sN /\ update_state_mods qc.mods sN s0 == sN /\ state_inv sN /\ k sN gN)
 
 [@va_qattr]
 let rec regs_match_file (r0:Regs.t) (r1:Regs.t) (rf:reg_file_id) (k:nat{k <= n_regs rf}) : Type0 =
@@ -371,6 +384,7 @@ unfold let wp_sound_code_pre (#a:Type0) (#c:code) (qc:quickCode a c) (s0:vale_st
 unfold let wp_sound_code_post (#a:Type0) (#c:code) (qc:quickCode a c) (s0:vale_state) (k:(s0':vale_state{s0 == s0'}) -> vale_state -> a -> Type0) ((sN:vale_state), (fN:fuel), (gN:a)) : Type0 =
   eval c s0 fN sN /\
   update_state_mods qc.mods sN s0 == sN /\
+  state_inv sN /\
   k s0 sN gN
 
 unfold let normal_steps : list string =
@@ -395,6 +409,6 @@ unfold let normal (x:Type0) : Type0 = norm [iota; zeta; simplify; primops; delta
 
 val wp_sound_code_norm (#a:Type0) (c:code) (qc:quickCode a c) (s0:vale_state) (k:(s0':vale_state{s0 == s0'}) -> vale_state -> a -> Type0) :
   Ghost (vale_state & fuel & a)
-    (normal (wp_sound_code_pre qc s0 k))
+    (t_require s0 /\ normal (wp_sound_code_pre qc s0 k))
     (wp_sound_code_post qc s0 k)
 
