vale/code/arch/x64/interop/Vale.Inline.X64.Fsqr_inline.fst
@@ -166,7 +166,7 @@ let fsqr_inline tmp f1 out =
     as_vale_buffer_len #TUInt64 #TUInt64 tmp;
     as_vale_buffer_len #TUInt64 #TUInt64 f1;
     as_vale_buffer_len #TUInt64 #TUInt64 out;
-    let x, _ = lowstar_fsqr_normal_t tmp f1 out () in
+    let (x, _) = lowstar_fsqr_normal_t tmp f1 out () in
     ()
 
 let fsqr_code_inline () : FStar.All.ML int =
@@ -268,7 +268,7 @@ let fsqr2_inline tmp f1 out =
     DV.length_eq (get_downview tmp);
     DV.length_eq (get_downview f1);
     DV.length_eq (get_downview out);
-    let x, _ = lowstar_fsqr2_normal_t tmp f1 out () in
+    let (x, _) = lowstar_fsqr2_normal_t tmp f1 out () in
     ()
 
 let fsqr2_code_inline () : FStar.All.ML int =
