vale/code/arch/x64/interop/Vale.Wrapper.X64.Fadd.fst
@@ -9,7 +9,7 @@ module DV = LowStar.BufferView.Down
 let add1 out f1 f2 =
   DV.length_eq (get_downview f1);
   DV.length_eq (get_downview out);
-  let x, _ = Vale.Stdcalls.X64.Fadd.add1 out f1 f2 () in
+  let (x, _) = Vale.Stdcalls.X64.Fadd.add1 out f1 f2 () in
   x
 
 #push-options "--max_fuel 0 --max_ifuel 0 --z3rlimit 100"
@@ -18,7 +18,7 @@ let fadd out f1 f2 =
   DV.length_eq (get_downview out);
   DV.length_eq (get_downview f1);
   DV.length_eq (get_downview f2);
-  let x, _ = Vale.Stdcalls.X64.Fadd.fadd_ out f1 f2 () in
+  let (x, _) = Vale.Stdcalls.X64.Fadd.fadd_ out f1 f2 () in
   ()
 
 #pop-options
